src/goose_lang/lib/typed_map/typed_map.v
@@ -1,6 +1,8 @@
 From iris.proofmode Require Import coq_tactics reduction.
 From Perennial.goose_lang Require Import notation proofmode typing.
-From Perennial.goose_lang.lib Require Import typed_mem.
+(* TODO: slice and struct imports are only to provide IntoVal instances, maybe
+should factor out IntoVal *)
+From Perennial.goose_lang.lib Require Import typed_mem slice.slice struct.struct.
 From Perennial.goose_lang.lib Require Import map.impl.
 From Perennial.goose_lang.lib Require map.map.
 Import uPred.
@@ -18,15 +20,6 @@ Class IntoValForType {ext V} (H: @IntoVal ext V) {ext_ty: ext_types ext} (t:ty) 
     { def_is_zero: to_val IntoVal_def = zero_val t;
       (* TODO: this isn't necessary, but it seems reasonable *)
       to_val_ty: forall v, val_ty (to_val v) t; }.
-
-Instance u64_IntoVal {ext: ext_op} : IntoVal u64 :=
-  {| to_val := λ (x: u64), LitV (LitInt x);
-     IntoVal_def := U64 0; |}.
-
-Instance u64_IntoVal_uint64T {ext} {ext_ty: ext_types ext} : IntoValForType u64_IntoVal uint64T.
-Proof.
-  constructor; auto.
-Qed.
 
 Module Map.
   Definition t V {ext} `{@IntoVal ext V} := gmap u64 V.
@@ -91,7 +84,7 @@ Ltac untype :=
 
 Theorem wp_NewMap stk E :
   {{{ True }}}
-    NewMap t @ stk; E
+    ref (zero_val (mapValT t)) @ stk; E
   {{{ mref, RET #mref;
       is_tmap mref ∅ }}}.
 Proof using IntoValForType0.
@@ -139,13 +132,22 @@ Proof.
   iApply (is_map_retype with "Hm").
 Qed.
 
-Theorem map_insert_fmap m k v' :
+Theorem map_insert_untype m k v' :
   map.map_insert (Map.untype m) k (to_val v') =
   Map.untype (map_insert m k v').
 Proof.
   untype.
   rewrite /map.map_insert /map_insert.
   rewrite fmap_insert //.
+Qed.
+
+Theorem map_del_untype m k :
+  map.map_del (Map.untype m) k =
+  Map.untype (map_del m k).
+Proof.
+  untype.
+  rewrite /map.map_del /map_del.
+  rewrite fmap_delete //.
 Qed.
 
 Theorem wp_MapInsert stk E mref m k v' vv :
@@ -160,8 +162,63 @@ Proof.
   wp_apply (map.wp_MapInsert with "Hm").
   iIntros "Hm".
   iApply "HΦ".
-  rewrite map_insert_fmap.
+  rewrite map_insert_untype.
+  iApply (is_map_retype with "Hm").
+Qed.
+
+Theorem wp_MapDelete stk E mref m k :
+  {{{ is_tmap mref m }}}
+    MapDelete #mref #k @ stk; E
+  {{{ RET #(); is_tmap mref (map_del m k) }}}.
+Proof.
+  iIntros (Φ) "Hm HΦ".
+  iDestruct (is_map_untype with "Hm") as "Hm".
+  wp_apply (map.wp_MapDelete with "Hm").
+  iIntros "Hm".
+  iApply "HΦ".
+  rewrite map_del_untype.
   iApply (is_map_retype with "Hm").
 Qed.
 
 End heap.
+
+Arguments wp_NewMap {_ _ _ _ _ _ _} V {_} {t}.
+Arguments wp_MapGet {_ _ _ _ _ _} V {_} {_ _}.
+Arguments wp_MapInsert {_ _ _ _ _ _} V {_} {_ _}.
+Arguments wp_MapDelete {_ _ _ _ _ _} V {_} {_ _}.
+
+(** instances for IntoVal *)
+Section instances.
+  Context {ext: ext_op} {ext_ty: ext_types ext}.
+  Global Instance u64_IntoVal : IntoVal u64 :=
+    {| to_val := λ (x: u64), #x;
+       IntoVal_def := U64 0; |}.
+
+  Global Instance u64_IntoVal_uint64T : IntoValForType u64_IntoVal uint64T.
+  Proof.
+    constructor; auto.
+  Qed.
+
+  Global Instance loc_IntoVal : IntoVal loc :=
+    {| to_val := λ (l: loc), #l;
+       IntoVal_def := null;
+    |}.
+
+  Global Instance loc_IntoVal_ref t : IntoValForType loc_IntoVal (struct.ptrT t).
+  Proof.
+    constructor; auto.
+  Qed.
+
+  Global Instance slice_IntoVal : IntoVal Slice.t :=
+    {| to_val := slice_val;
+       IntoVal_def := Slice.nil;
+    |}.
+
+  Global Instance slice_IntoVal_ref t : IntoValForType slice_IntoVal (slice.T t).
+  Proof.
+    constructor; auto.
+    intros.
+    apply slice_val_ty.
+  Qed.
+
+End instances.
